## Arcusfunktioner

Inverser till sinus, cosinus, tangens mm.

### Arcsin
Inversen till $y=\sin{x}$  $- \frac{\pi}{2}\le x\le \frac{\pi}{2}$  
kallas arcsinus ($\sin^{-1}x$)  
$y=\arcsin{x}$  
$\Leftrightarrow$  
$x=\sin{y}$,  $- \frac{\pi}{2}\le x\le \frac{\pi}{2}$  

Kanceleringslagar  
$\arcsin(\sin(x))=x$,  $- \frac{\pi}{2}\le x\le \frac{\pi}{2}$  
$\sin(\arcsin(x))=x$,  $-1\le x\le 1$  

#### Derivatan
$y=\arcsin(x) \Leftrightarrow\sin{y}=x$  
$\frac{d}{dx}\sin{y}=\frac{d}{dx}(x)$  
$\cos(y)-y'=1$  
$y'=\frac{1}{\cos{y}}$,  $- \frac{\pi}{2}\le y\le \frac{\pi}{2}$  

![](sin-Drawing2023-10-0314.05.18.excalidraw.svg)  

$\cos{y}=\sqrt{1^{2}-x^{2}}=\sqrt{1-x^{2}}$  

$\frac{d}{dx}(\arcsin{x})=\frac{1}{\sqrt{1-x^{2}}}$  

### Arctan
$\tan(x)$,  $- \frac{\pi}{2}\le x\le \frac{\pi}{2}$  
$\frac{d}{dx}(\tan(x))=\frac{1}{\cos^{2}x}=(1+\tan^{2}x)>0$ på $(- \frac{\pi}{2}, \frac{\pi}{2})$  

$\tan{x}$ är 1-1
Inversen kallas arctangens  
$y=\arctan(x) \Leftrightarrow \tan(y)=x$,  $- \frac{\pi}{2}\le y \le \frac{\pi}{2}$  
$\arctan(\tan(x))=x$,  $- \frac{\pi}{2}\le x \le \frac{\pi}{2}$  
$\tan(\arctan(x))=x$,  $-\infty<x<\infty$   

#### Derivatan
$y=\arctan(x) \Leftrightarrow \tan{y}=x$  
Implicit derivering
$\frac{d}{dx}(\tan{y})=\frac{d}{dx}(x)$  
$(1+\tan^{2}{y})y'=1$  
![](tan-Drawing2023-10-0314.05.18.excalidraw.svg)  

$\tan(y)=\frac{x}{1}=x$  
$1+\tan^{2}(y)=1+x^{2}$  
$y'=\frac{1}{1+\tan^{2}(y)}$  
$y'=\frac{1}{1+x^{2}}$  

### Arccos
$\cos(y)=\sin(\frac{\pi}{2}-y)$,  $0\le y\le \pi$  

Inversen av $\cos(x)$,  $0\le y\le \pi$  
kallas arcuscosinus ($\arccos(x)$)  

$y=\arccos(x)\Leftrightarrow \cos{y}=x$,  $0\le y\le \pi$  
$\sin(\frac{\pi}{2}-y)=x$  
$\Leftrightarrow$  
$\frac{\pi}{2}-y=\arcsin{x}$  
$y=\arccos{x}$ ger att  
$\frac{\pi}{2}-\arccos{x}=\arcsin{x}$  
$\Leftrightarrow$  
$\arccos{x}=\frac{\pi}{2}-\arcsin{x}$,  $-1\le x\le 1$  

#### Derivatan
$\frac{d}{dx}(\arccos{x})=\frac{-1}{\sqrt{1-x^{2}}}$  

$\frac{d}{dx}\arccos(x)=\frac{d}{dx}(\frac{\pi}{2})-\frac{d}{dx}(\arcsin{x})$  
$=0-\frac{1}{\sqrt{1-x^{2}}}=-\frac{1}{1-x^{2}}$  
