1.38
visa att för alla $n\in\mathbb{Z}_{+}$ gäller:  
$1^{2}-2^{2}+3^{2}-4^{2}+..+(-1)^{n-1}n^{2}=(-1)^{n+1}\frac{n(n+1)}{2}$  

> 1.   
>   $1^{2}=1$  
>   $(-1)^{1+1}\frac{1(1+1)}{2}=1$  
>   $VL=HL$  
>   
> 2.  
>   $P_{k}=1^{2}-2^{2}+3^{2}-4^{2}+..+(-1)^{k-1}k^{2}=(-1)^{k+1}\frac{k(k+1)}{2}$  
>   $P_{k+1}$ ska bli lika med $(-1)^{(k+1)+1}\frac{(k+1)((k+1)+1)}{2}=(-1)^{k+2}\frac{k(k+2)+(k+2)}{2}=(-1)^{k}\frac{k(k+2)+(k+2)}{2}$
>   $=(-1)^{k}\frac{k^2+3k+2}{2}$
>   $P_{k+1}=1^{2}-2^{2}+3^{2}-4^{2}+..+(-1)^{k-1}k^{2}+(-1)^{(k+1)-1}(k+1)^{2}$  
>   $=(-1)^{k+1}\frac{k(k+1)}{2}+(-1)^{(k+1)-1}(k+1)^{2}$  
>   $=(-1)^{k+1}\frac{k(k+1)}{2}+(-1)^{k}\frac{2(k+1)^{2}}{2}$  
>   $=\frac{(-1)^{k+1}k(k+1)+(-1)^{k}2(k+1)^{2}}{2}$  
>   $=(-1)^{k}\frac{(-1)^{1}k(k+1)+2(k+1)^2}{2}$  
>   $=(-1)^k\frac{-(k^{2}+k)+2(k^2+2k+1)}{2}=(-1)^{k}\frac{k^{2}+3k+2}{2}=HL$  


1.40  
visa att $1+\frac{1}{\sqrt{2}}+\frac{1}{\sqrt{3}}+..+\frac{1}{\sqrt{n}}\ge\sqrt{n}$  

> 